LF to Hyb is weird

LanguagesEquivalence/LF_to_Hyb.v
@@ -13,6 +13,8 @@ Open Scope is5_scope.
 Open Scope permut_scope.
 Open Scope hybrid_is5_scope.
 
+(* Relation for contexts *)
+
 Definition LF_to_Hyb_ctx (G: bg_LF) (G': bg_Hyb) :=
   PPermut_LF (map snd_ G') G /\ ok_Hyb G' nil.
 
@@ -118,22 +120,16 @@ apply LF_to_Hyb_PPermut_LF_bg with (G:=y); auto;
 apply LF_to_Hyb_PPermut_Hyb_bg with (G':=y0); auto.
 Qed.
 
-Fixpoint LF_to_Hyb_ctx_fun (G: bg_LF) (U: list var) :=
-match G with
-| nil => nil
-| Gamma :: G' =>
-  let w:= var_gen (from_list U) in
-  (w, Gamma) :: LF_to_Hyb_ctx_fun G' (w::U)
-end.
+(* Relation for typing terms *)
 
-Inductive LF_to_Hyb_rel: ctx_LF  -> te_LF  -> ty ->
+Inductive LF_to_Hyb_term_R: ctx_LF  -> te_LF  -> ty ->
                          bg_Hyb -> var -> te_Hyb -> Prop :=
 
 | hyp_LF_Hyb:
     forall G Gamma G' w v A,
       types_LF G Gamma (hyp_LF v) A ->
       LF_to_Hyb_ctx (Gamma::G) ((w, Gamma)::G') ->
-      LF_to_Hyb_rel Gamma (hyp_LF v) A
+      LF_to_Hyb_term_R Gamma (hyp_LF v) A
                     G' w (hyp_Hyb v)
 
 | lam_LF_Hyb:
@@ -142,34 +138,34 @@ Inductive LF_to_Hyb_rel: ctx_LF  -> te_LF  -> ty ->
       LF_to_Hyb_ctx (Gamma::G) ((w, Gamma)::G') ->
       (forall v0,
          v0 \notin L ->
-         LF_to_Hyb_rel ((v0, A)::Gamma) (open_LF M (hyp_LF (fte v0))) B
+         LF_to_Hyb_term_R ((v0, A)::Gamma) (open_LF M (hyp_LF (fte v0))) B
                        G' w
                        (M' ^t^ (hyp_Hyb (fte v0)))) ->
-      LF_to_Hyb_rel Gamma (lam_LF A M) (A ---> B) G' w (lam_Hyb A M')
+      LF_to_Hyb_term_R Gamma (lam_LF A M) (A ---> B) G' w (lam_Hyb A M')
 
 | appl_LF_Hyb:
     forall G Gamma G' w M1 M2 N1 N2 A B,
       types_LF G Gamma (appl_LF M1 N1) B ->
-      LF_to_Hyb_rel Gamma M1 (A ---> B) G' w M2 ->
-      LF_to_Hyb_rel Gamma N1 A G' w N2 ->
+      LF_to_Hyb_term_R Gamma M1 (A ---> B) G' w M2 ->
+      LF_to_Hyb_term_R Gamma N1 A G' w N2 ->
       LF_to_Hyb_ctx (Gamma::G) ((w, Gamma)::G') ->
-      LF_to_Hyb_rel Gamma (appl_LF M1 N1) B G' w (appl_Hyb M2 N2)
+      LF_to_Hyb_term_R Gamma (appl_LF M1 N1) B G' w (appl_Hyb M2 N2)
 
 | box_LF_Hyb:
     forall L G Gamma G' w M N A,
       types_LF G Gamma (box_LF M) ([*]A) ->
       LF_to_Hyb_ctx (Gamma::G) ((w, Gamma)::G') ->
       (forall w0, w0 \notin L ->
-        LF_to_Hyb_rel (@nil (var*ty)) M A
+        LF_to_Hyb_term_R (@nil (var*ty)) M A
                       ((w,Gamma)::G') w0 (N ^w^ (fwo w0))) ->
-      LF_to_Hyb_rel Gamma (box_LF M) ([*]A) G' w (box_Hyb N)
+      LF_to_Hyb_term_R Gamma (box_LF M) ([*]A) G' w (box_Hyb N)
 
 | unbox_LF_Hyb:
     forall G Gamma G' w M N A,
       types_LF G Gamma (unbox_LF M) A ->
       LF_to_Hyb_ctx (Gamma::G) ((w, Gamma)::G') ->
-      LF_to_Hyb_rel Gamma M ([*]A) G' w N ->
-      LF_to_Hyb_rel Gamma (unbox_LF M) A
+      LF_to_Hyb_term_R Gamma M ([*]A) G' w N ->
+      LF_to_Hyb_term_R Gamma (unbox_LF M) A
                     G' w (unbox_fetch_Hyb (fwo w) N)
 
 | unbox_fetch_LF_Hyb:
@@ -177,18 +173,18 @@ Inductive LF_to_Hyb_rel: ctx_LF  -> te_LF  -> ty ->
       w <> w' ->
       types_LF (Gamma'::G) Gamma (unbox_LF M) A ->
       LF_to_Hyb_ctx (Gamma::Gamma'::G) ((w, Gamma)::(w', Gamma')::G') ->
-      LF_to_Hyb_rel Gamma' M ([*]A)
+      LF_to_Hyb_term_R Gamma' M ([*]A)
                     ((w, Gamma)::G') w' N ->
       ((w', Gamma')::G') ~=~ G'' ->
-      LF_to_Hyb_rel Gamma (unbox_LF M) A
+      LF_to_Hyb_term_R Gamma (unbox_LF M) A
                     G'' w (unbox_fetch_Hyb (fwo w') N)
 
 | here_LF_Hyb:
     forall G Gamma G' w A M N,
       types_LF G Gamma (here_LF M) (<*>A) ->
       LF_to_Hyb_ctx (Gamma::G) ((w, Gamma)::G') ->
-      LF_to_Hyb_rel Gamma M A G' w N ->
-      LF_to_Hyb_rel Gamma (here_LF M) (<*>A)
+      LF_to_Hyb_term_R Gamma M A G' w N ->
+      LF_to_Hyb_term_R Gamma (here_LF M) (<*>A)
                     G' w (get_here_Hyb (fwo w) N)
 
 | get_here_LF_Hyb:
@@ -196,46 +192,46 @@ Inductive LF_to_Hyb_rel: ctx_LF  -> te_LF  -> ty ->
       w <> w' ->
       types_LF (Gamma'::G) Gamma (here_LF M) (<*>A) ->
       LF_to_Hyb_ctx (Gamma::Gamma'::G) ((w, Gamma)::(w', Gamma')::G') ->
-      LF_to_Hyb_rel Gamma' M A
+      LF_to_Hyb_term_R Gamma' M A
                     ((w, Gamma)::G') w' N ->
       ((w', Gamma')::G') ~=~ G'' ->
-      LF_to_Hyb_rel Gamma (here_LF M) (<*>A)
+      LF_to_Hyb_term_R Gamma (here_LF M) (<*>A)
                     G'' w (get_here_Hyb (fwo w') N)
 
 | letdia_LF_Hyb:
     forall Lt Lw G Gamma G' w A B M1 M2 N1 N2,
       types_LF G Gamma (letdia_LF M1 N1) B ->
-      LF_to_Hyb_rel Gamma M1 (<*>A) G' w M2 ->
+      LF_to_Hyb_term_R Gamma M1 (<*>A) G' w M2 ->
       (forall w'0 v', w'0 \notin Lw -> v' \notin Lt ->
-                     LF_to_Hyb_rel Gamma (open_LF N1 (hyp_LF (fte v'))) B
+                     LF_to_Hyb_term_R Gamma (open_LF N1 (hyp_LF (fte v'))) B
                                    ((w'0, (v', A) :: nil ) :: G') w
                                    ((N2 ^w^ fwo w'0 ) ^t^ hyp_Hyb (fte v'))) ->
       LF_to_Hyb_ctx (Gamma::G) ((w, Gamma)::G') ->
-      LF_to_Hyb_rel Gamma (letdia_LF M1 N1) B G' w
+      LF_to_Hyb_term_R Gamma (letdia_LF M1 N1) B G' w
                     (letdia_get_Hyb (fwo w) M2 N2)
 
 | letdia_get_LF_Hyb:
     forall Lt Lw G Gamma Gamma' G' w w' A B M1 M2 N1 N2 G'',
       types_LF (Gamma'::G) Gamma (letdia_LF M1 N1) B ->
-      LF_to_Hyb_rel Gamma' M1 (<*>A)
+      LF_to_Hyb_term_R Gamma' M1 (<*>A)
                     ((w, Gamma)::G') w' M2 ->
       (forall w'0 v', w'0 \notin Lw -> v' \notin Lt ->
-         LF_to_Hyb_rel Gamma (open_LF N1 (hyp_LF (fte v'))) B
+         LF_to_Hyb_term_R Gamma (open_LF N1 (hyp_LF (fte v'))) B
                        (((w'0, (v', A) :: nil ) :: (w', Gamma')::G'))
                        w ((N2 ^w^ fwo w'0 ) ^t^ hyp_Hyb (fte v'))) ->
       LF_to_Hyb_ctx (Gamma::Gamma'::G) ((w, Gamma)::(w', Gamma')::G') ->
       (w', Gamma')::G' ~=~ G'' ->
-      LF_to_Hyb_rel Gamma (letdia_LF M1 N1) B
+      LF_to_Hyb_term_R Gamma (letdia_LF M1 N1) B
                     G'' w
                     (letdia_get_Hyb (fwo w') M2 N2)
 .
 
-Lemma LF_to_Hyb_rel_permut_G_Gamma:
+Lemma LF_to_Hyb_term_R_permut_G_Gamma:
 forall Gamma Gamma' M A G w M' G',
   Gamma *=* Gamma' ->
   G ~=~ G' ->
-  LF_to_Hyb_rel Gamma M A G w M' ->
-  LF_to_Hyb_rel Gamma' M A G' w M'.
+  LF_to_Hyb_term_R Gamma M A G w M' ->
+  LF_to_Hyb_term_R Gamma' M A G' w M'.
 intros; generalize dependent G'; generalize dependent Gamma';
 induction H1; intros; try econstructor; eauto.
 rewrite <- H1; eauto.
@@ -300,16 +296,18 @@ rewrite <- HP1; rewrite <- HP2; eauto.
 rewrite <- H6; rewrite H4; auto.
 Qed.
 
-Add Morphism LF_to_Hyb_rel: LF_to_Hyb_rel_G.
+Add Morphism LF_to_Hyb_term_R: LF_to_Hyb_term_R_G.
 split; intros.
-eapply LF_to_Hyb_rel_permut_G_Gamma with (G:=x0) (Gamma:=x); auto.
-eapply LF_to_Hyb_rel_permut_G_Gamma with (G:=y2) (Gamma:=y); auto; symmetry;
+eapply LF_to_Hyb_term_R_permut_G_Gamma with (G:=x0) (Gamma:=x); auto.
+eapply LF_to_Hyb_term_R_permut_G_Gamma with (G:=y2) (Gamma:=y); auto; symmetry;
 auto.
 Qed.
 
+(* .. it types! *)
+
 Lemma LF_to_Hyb_types:
 forall G' Gamma M A w M',
-  LF_to_Hyb_rel Gamma M A G' w M' ->
+  LF_to_Hyb_term_R Gamma M A G' w M' ->
   types_Hyb G' (w, Gamma) M' A.
 intros; induction H; intros.
 (* hyp *)
@@ -422,13 +420,86 @@ rewrite <- H7; eauto.
 PPermut_Hyb_simpl.
 Qed.
 
+(* ...it preserves values! *)
+
 Lemma LF_to_Hyb_value:
 forall G' Gamma M A w M',
-  LF_to_Hyb_rel Gamma M A G' w M' ->
+  LF_to_Hyb_term_R Gamma M A G' w M' ->
   value_LF M -> value_Hyb M'.
 intros; induction H; simpl;
 inversion H0; subst; constructor; eauto.
 Qed.
+
+Lemma L_to_Hyb_subst_t:
+forall M M' N N' G Gamma' G' Gamma w w' B A v,
+  LF_to_Hyb_term_R Gamma N B G w N' ->
+  LF_to_Hyb_term_R Gamma' M A G' w' M' ->
+  (* inner subst *)
+  ((w, Gamma) :: G ~=~ (w', (v, A) :: Gamma') :: G' ->
+   LF_to_Hyb_term_R Gamma' (subst_t_LF M (fte v) N) B G w ([M'//(fte v)]N')) /\
+  (* outer subst *) True.
+Admitted.
+(*
+intros. generalize dependent N; generalize dependent N'.
+remember  ((v, A1) :: Gamma) as Gamma';
+generalize dependent Gamma;
+generalize dependent v;
+generalize dependent A1.
+induction H; intros; simpl in *; subst.
+inversion H; subst; repeat case_if.
+inversion H2; subst.
+rewrite Mem_cons_eq in H5; destruct H5.
+inversion H4; subst; auto.
+skip. (* Ok + H4 = contradiction *)
+econstructor; eauto. constructor; eauto. skip. skip. skip. (*trivial *)
+(* lam *)
+econstructor; eauto.
+replace (lam_LF A (subst_t_LF N (fte v) M)) with
+(subst_t_LF N (fte v) (lam_LF A M)).
+apply subst_t_LF_preserv_types_inner with (A:=A1). skip. eauto.
+skip. simpl; auto. skip.
+intros. unfold open_LF in *.
+rewrite <- subst_t_comm_LF. unfold open_t_Hyb in *.
+rewrite <- subst_t_Hyb_comm. apply H2 with (A2:=A1); eauto.
+skip. (* permut *) skip. (* weakening *) skip. skip. skip. skip.
+Admitted.
+*)
+
+Lemma L_to_Hyb_subst_t_inner:
+forall M M' N N' G Gamma w B A v,
+  LF_to_Hyb_term_R ((v, A)::Gamma) N B G w N' ->
+  LF_to_Hyb_term_R Gamma M A G w M' ->
+  LF_to_Hyb_term_R Gamma (subst_t_LF M (fte v) N) B G w ([M'//(fte v)]N').
+intros; eapply L_to_Hyb_subst_t
+        with (Gamma':=Gamma) (Gamma:=(v, A)::Gamma); eauto.
+Qed.
+
+(* Can it also preserve reductions? *)
+
+Lemma L_to_Hyb_step:
+forall M M' G' Gamma N w A,
+  lc_w_Hyb N ->
+  LF_to_Hyb_term_R Gamma M A G' w N -> step_LF M M' ->
+  exists N', LF_to_Hyb_term_R Gamma M' A G' w N' /\
+             step_Hyb (N, fwo w) (N', fwo w).
+induction M; intros; inversion H1; subst.
+(* appl_lam *)
+clear IHM1 IHM2.
+inversion H0; inversion H7; subst.
+exists (M' ^t^ N2); split.
+unfold open_t_Hyb in *; unfold open_LF in *.
+assert (exists x, x \notin L \u used_vars_te_LF M \u free_vars_Hyb M')
+  by apply Fresh; destruct H2.
+rewrite subst_t_neutral_free_LF with (v:=x); auto.
+rewrite subst_t_Hyb_neutral_free with (v:=x); auto.
+apply L_to_Hyb_subst_t_inner with (A:=A1); eauto.
+econstructor; auto.
+skip. skip. skip. skip. (* lc * *)
+(* appl *)
+Admitted.
+
+(*
+(* Simpler relation that captures too much -- but preserves it all! *)
 
 (* Fixme: rename if this works and stays (being useful) *)
 Inductive R: te_LF -> te_Hyb -> Prop :=
@@ -491,48 +562,6 @@ induction M; intros; inversion H; destruct N; simpl in *;
 inversion H2; subst; inversion H; subst; constructor; eauto.
 induction M; intros; inversion H; subst; simpl in *; repeat case_if;
 constructor; eauto.
-Qed.
-
-(* This simply states that LF_to_Hyb_rel is one realisation of R *)
-Lemma LF_to_Hyb_rel_R:
-forall M1 Gamma A G' w M2,
-  LF_to_Hyb_rel Gamma M1 A G' w M2 ->
-  R M1 M2.
-intros; induction H; constructor; auto.
-(* lam *)
-assert (exists x, x\notin L \u  used_vars_te_LF M \u free_vars_Hyb M')
-  by apply Fresh; destruct H3;
-specialize H2 with x;
-unfold open_LF in *; unfold open_t_Hyb in *; apply R_subst_t_rev in H2; auto.
-(* box *)
-assert (exists x, x\notin L) by apply Fresh; destruct H3;
-unfold open_w_Hyb in *. eapply R_subst_w; eauto.
-(* letdia *)
-assert (exists x, x\notin Lw) by apply Fresh.
-destruct H4.
-assert (exists x0, x0 \notin Lt \u used_vars_te_LF N1 \u
-                              free_vars_Hyb {{fwo x // bwo 0}}N2)
-  by apply Fresh; destruct H5.
-specialize H2 with x x0.
-unfold open_LF in *; unfold open_t_Hyb in *;
-unfold open_w_Hyb in *.
-apply H2 in H4; auto.
-assert (R N1 ({{fwo x // bwo 0}} N2)).
-apply R_subst_t_rev with (v:=0) (v':=x0); eauto.
-apply R_subst_w with (w:=fwo x) (w':=bwo 0); auto.
-(* letdia - get *)
-assert (exists x, x\notin Lw) by apply Fresh.
-destruct H5.
-assert (exists x0, x0 \notin Lt \u used_vars_te_LF N1 \u
-                              free_vars_Hyb {{fwo x // bwo 0}}N2)
-  by apply Fresh; destruct H6.
-specialize H2 with x x0.
-unfold open_LF in *; unfold open_t_Hyb in *;
-unfold open_w_Hyb in *.
-apply H2 in H5; auto.
-assert (R N1 ({{fwo x // bwo 0}} N2)).
-apply R_subst_t_rev with (v:=0) (v':=x0); eauto.
-apply R_subst_w with (w:=fwo x) (w':=bwo 0); auto.
 Qed.
 
 Lemma R_lc_t:
@@ -611,8 +640,55 @@ intros; induction H; simpl in *;
 try rewrite IHR || (rewrite IHR1; rewrite IHR2); eauto.
 Qed.
 
-(* End of R properties *)
+(* This simply states that LF_to_Hyb_term_R is one realisation of R *)
+Lemma LF_to_Hyb_term_R_R:
+forall M1 Gamma A G' w M2,
+  LF_to_Hyb_term_R Gamma M1 A G' w M2 ->
+  R M1 M2.
+intros; induction H; constructor; auto.
+(* lam *)
+assert (exists x, x\notin L \u  used_vars_te_LF M \u free_vars_Hyb M')
+  by apply Fresh; destruct H3;
+specialize H2 with x;
+unfold open_LF in *; unfold open_t_Hyb in *; apply R_subst_t_rev in H2; auto.
+(* box *)
+assert (exists x, x\notin L) by apply Fresh; destruct H3;
+unfold open_w_Hyb in *. eapply R_subst_w; eauto.
+(* letdia *)
+assert (exists x, x\notin Lw) by apply Fresh.
+destruct H4.
+assert (exists x0, x0 \notin Lt \u used_vars_te_LF N1 \u
+                              free_vars_Hyb {{fwo x // bwo 0}}N2)
+  by apply Fresh; destruct H5.
+specialize H2 with x x0.
+unfold open_LF in *; unfold open_t_Hyb in *;
+unfold open_w_Hyb in *.
+apply H2 in H4; auto.
+assert (R N1 ({{fwo x // bwo 0}} N2)).
+apply R_subst_t_rev with (v:=0) (v':=x0); eauto.
+apply R_subst_w with (w:=fwo x) (w':=bwo 0); auto.
+(* letdia - get *)
+assert (exists x, x\notin Lw) by apply Fresh.
+destruct H5.
+assert (exists x0, x0 \notin Lt \u used_vars_te_LF N1 \u
+                              free_vars_Hyb {{fwo x // bwo 0}}N2)
+  by apply Fresh; destruct H6.
+specialize H2 with x x0.
+unfold open_LF in *; unfold open_t_Hyb in *;
+unfold open_w_Hyb in *.
+apply H2 in H5; auto.
+assert (R N1 ({{fwo x // bwo 0}} N2)).
+apply R_subst_t_rev with (v:=0) (v':=x0); eauto.
+apply R_subst_w with (w:=fwo x) (w':=bwo 0); auto.
+Qed.
 
+(*****************************************************************************)
+(* LF_to_Hyb_term_R is left-total for typing terms
+I just want to "see what it takes" to proove this, not really make a full proof.
+ *)
+
+(* We can replace one variable with another in the environment and the term
+ -- and the typing is intact *)
 Fixpoint subst_in_ctx_LF (v1: var) (v2: var) (Gamma: ctx_LF) : ctx_LF :=
 match Gamma with
 | nil => nil
@@ -661,27 +737,18 @@ rewrite <- IHG; eauto.
 simpl; auto.
 Qed.
 
-Lemma ok_Bg_LF_subst_in_bg_subst_in_ctx:
-forall G G' Gamma w v1 v,
-LF_to_Hyb_ctx (Gamma :: G) ((w, Gamma) :: G') ->
-ok_Bg_LF (subst_in_ctx_LF v1 v Gamma ::
-                          map (subst_in_ctx_LF v1 v) G).
-Admitted.
-
 Lemma Mem_ctx_LF:
-forall v v' v0 v1 A Gamma,
+forall Gamma v v' v0 v1 A,
   Mem (v, A) Gamma ->
   (v' = if (eq_var_dec v v0) then v1 else v) ->
   Mem (v', A) (subst_in_ctx_LF v1 v0 Gamma).
-Admitted.
-
-Lemma LF_to_Hyb_ctx_subst_t:
-forall Gamma G w G' v0 v1,
-LF_to_Hyb_ctx (Gamma :: G) ((w, Gamma) :: G') ->
-LF_to_Hyb_ctx
-     (subst_in_ctx_LF v1 v0 Gamma :: map (subst_in_ctx_LF v1 v0) G)
-     ((w, subst_in_ctx_LF v1 v0 Gamma) :: map (subst_in_ctx_Hyb v1 v0) G').
-Admitted.
+induction Gamma; intros; [rewrite Mem_nil_eq in *; contradiction | ];
+destruct a; rewrite Mem_cons_eq in *. simpl.
+destruct H.
+inversion H; subst; case_if; apply Mem_here.
+repeat case_if; rewrite Mem_cons_eq; right; eapply IHGamma; eauto;
+case_if; auto.
+Qed.
 
 Lemma types_renaming:
 forall G Gamma M B v0 v,
@@ -692,271 +759,105 @@ forall G Gamma M B v0 v,
 intros; generalize dependent v; generalize dependent v0; induction H; intros.
 Admitted.
 
-Lemma LF_to_Hyb_rel_rename_vars:
+Lemma LF_to_Hyb_term_R_rename_vars:
 forall Gamma M B G w N v,
-  LF_to_Hyb_rel Gamma M B G w N ->
+  LF_to_Hyb_term_R Gamma M B G w N ->
   forall v0 Gamma' G' M' N',
     v0 \notin \{} ->
     Gamma' = subst_in_ctx_LF v0 v Gamma ->
     G' = map (subst_in_ctx_Hyb v0 v) G ->
     M' = subst_t_LF (hyp_LF (fte v0)) (fte v) M ->
     N' = subst_t_Hyb (hyp_Hyb (fte v0)) (fte v) N ->
-    LF_to_Hyb_rel Gamma' M' B G' w N'.
-intros Gamma M B G w N v H; generalize dependent v;
-induction H; intros; subst; simpl in *; repeat case_if.
-(* hyp *)
-apply hyp_LF_Hyb with (G:=map (subst_in_ctx_LF v1 v0) G); inversion H; subst.
-constructor;
-[eapply ok_Bg_LF_subst_in_bg_subst_in_ctx |
- apply Mem_ctx_LF with (v:=v0); auto; case_if]; eauto.
-apply LF_to_Hyb_ctx_subst_t; auto.
-apply hyp_LF_Hyb with (G:=map (subst_in_ctx_LF v1 v0) G); inversion H; subst.
-constructor;
-[eapply ok_Bg_LF_subst_in_bg_subst_in_ctx |
- apply Mem_ctx_LF with (v:=v2); auto; case_if]; eauto.
-apply LF_to_Hyb_ctx_subst_t; auto.
-(* lam *)
-apply lam_LF_Hyb with (L:=L \u \{v}) (G:=map (subst_in_ctx_LF v0 v) G);
-inversion H; subst.
-apply t_lam_LF with (L:=L0 \u L \u \{v});
-[eapply ok_Bg_LF_subst_in_bg_subst_in_ctx | intros]; eauto.
-replace ((v1, A) :: subst_in_ctx_LF v0 v Gamma) with
-  (subst_in_ctx_LF v0 v ((v1, A)::Gamma)).
-unfold open_LF. rewrite <- subst_t_comm_LF; try constructor; eauto.
-apply types_renaming; eauto.
-simpl; case_if; auto; repeat rewrite notin_union in H4;
-rewrite notin_singleton in H4; destruct H4; destruct H5; elim H6; auto.
-apply LF_to_Hyb_ctx_subst_t; auto.
-intros. apply H2 with (v0:=v1)(v1:=v0)(v:=v); eauto; repeat case_if; auto.
-rewrite notin_union in *; destruct H4; rewrite notin_singleton in *;
-elim H5; auto.
-unfold open_LF; rewrite subst_t_comm_LF; auto; constructor.
-unfold open_t_Hyb; rewrite subst_t_Hyb_comm; auto; constructor.
-(* appl *)
+    LF_to_Hyb_term_R Gamma' M' B G' w N'.
 Admitted.
 
-Definition subst_w_in_ctx_Hyb w1 w2 (Gamma: ctx_Hyb) :=
-let w' :=  if eq_var_dec (fst_ Gamma) w2 then w1 else (fst_ Gamma)
-in (w', snd_ Gamma).
+Lemma subst_t_Hyb_neutral_bound:
+forall (M : te_Hyb) x y k,
+  lc_t_n_Hyb k M ->
+  [hyp_Hyb (fte x)//fte y]M =
+  [hyp_Hyb (fte x) // bte k]([hyp_Hyb (bte k) // fte y]M).
+induction M; intros; simpl in *; repeat (case_if; simpl in * ); auto.
+inversion H; omega.
+inversion H; subst; rewrite IHM with (k:=S k); auto.
+Admitted. (* This is not true in current implementation of substitution! *)
 
-Lemma subst_w_in_bg_Hyb_no_change:
-forall G v1 v2,
-  v2 \notin from_list (map fst_ G) ->
-  G = map (subst_w_in_ctx_Hyb v1 v2) G.
-unfold subst_w_in_ctx_Hyb in *;
-induction G; intros; rew_map; auto;
-destruct a; rew_map in *; simpl in *; case_if;
-rewrite from_list_cons in H; rewrite notin_union in H; destruct H.
-elim H; rewrite in_singleton; auto.
-rewrite <- IHG; eauto.
-Qed.
-
-Lemma LF_to_Hyb_rel_rename_worlds:
-forall Gamma M B G N w w'',
-  LF_to_Hyb_rel Gamma M B G w N ->
-  forall w' G' N' w0,
-    w' \notin \{} ->
-    G' = map (subst_w_in_ctx_Hyb w' w'') G ->
-    N' = subst_w_Hyb (fwo w') (fwo w'') N ->
-    (w0 = if (eq_var_dec w w'') then w' else w) ->
-    LF_to_Hyb_rel Gamma M B G' w0 N'.
-Admitted.
-
-Lemma LF_to_Hyb_rel_lc_t:
-forall Gamma M A G w N',
-  LF_to_Hyb_rel Gamma M A G w N' ->
-  lc_t_Hyb N'.
+Lemma LF_to_Hyb_term_R_renaming:
+forall G' Gamma x A B NtoX v0 w M,
+lc_t_Hyb NtoX ->
+x \notin from_list (map fst_ Gamma) \u
+  vars_from_G_Hyb G'\u used_vars_te_LF M ->
+LF_to_Hyb_term_R ((x, A) :: Gamma)
+         (subst_t_LF (hyp_LF (fte x)) (bte 0) M) B G' w NtoX ->
+LF_to_Hyb_term_R ((v0, A) :: Gamma)
+                 (subst_t_LF (hyp_LF (fte v0)) (bte 0) M) B G' w
+                 [hyp_Hyb (fte v0) // bte 0]([hyp_Hyb (bte 0) // fte x]NtoX).
 intros.
-apply types_Hyb_lc_t_Hyb with (G:=G) (Gamma:=Gamma) (A:=A) (w:=w).
-apply LF_to_Hyb_types in H; auto.
+apply LF_to_Hyb_term_R_rename_vars with (v:=x) (v0:=v0)
+                                        (Gamma':=(v0,A)::Gamma)
+                                        (G':=G')
+(M':=subst_t_LF (hyp_LF (fte v0)) (bte 0) M)
+(N':=[hyp_Hyb (fte v0) // bte 0]([hyp_Hyb (bte 0) // fte x]NtoX)) in H1;
+auto.
+simpl; case_if; rewrite subst_in_ctx_LF_no_change; auto.
+rewrite <- subst_in_bg_Hyb_no_change; auto.
+rewrite <- subst_t_neutral_free_LF; auto.
+rewrite subst_t_Hyb_neutral_bound with (k:=0); auto.
 Qed.
 
-Lemma LF_to_Hyb_rel_subst_t_rev:
-forall N Gamma M v N' A B G w M',
-  LF_to_Hyb_rel Gamma (subst_t_LF M v N) A G w N' ->
-  LF_to_Hyb_rel Gamma M B G w M' ->
-  exists N0,
-    N' = subst_t_Hyb M' v N0.
-induction N; intros; simpl in *; repeat case_if.
-Admitted.
-
-Lemma LF_to_Hyb_rel_te_vars:
-forall N1 N2 Gamma A G w,
-  LF_to_Hyb_rel Gamma N1 A G w N2 ->
-  used_vars_te_LF N1 = free_vars_Hyb N2.
-intros; apply R_te_vars; eapply LF_to_Hyb_rel_R; eauto.
-Qed.
-
-Lemma free_vars_Hyb_subst_t:
-forall N C k,
-  free_vars_Hyb ([C // bte k] N) = free_vars_Hyb N \/
-  free_vars_Hyb ([C // bte k] N) = free_vars_Hyb C \u free_vars_Hyb N.
-induction N; intros; simpl in *.
-destruct v; case_if; simpl;
-[right; rewrite union_empty_r | left | left ]; auto.
-destruct IHN with C (S k); rewrite <- H; [left | right]; auto.
-destruct IHN1 with C k; destruct IHN2 with C k; rewrite H; rewrite H0;
-[left | right | right | right]; auto.
-rewrite <- union_comm_assoc; auto.
-rewrite union_assoc; auto.
-rewrite <- union_comm_assoc.
-rewrite <- union_assoc.
-assert (forall N,
-          free_vars_Hyb C \u free_vars_Hyb C \u N = free_vars_Hyb C \u N).
-intros; rewrite union_assoc; rewrite union_same; auto.
-rewrite H1; auto.
-destruct IHN with C k; rewrite H; [left | right]; auto.
-destruct IHN with C k; rewrite H; [left | right]; auto.
-destruct IHN with C k; rewrite H; [left | right]; auto.
-destruct IHN1 with C k; destruct IHN2 with C (S k); rewrite H; rewrite H0;
-[left | right | right | right]; auto.
-rewrite <- union_comm_assoc; auto.
-rewrite union_assoc; auto.
-rewrite <- union_comm_assoc.
-rewrite <- union_assoc.
-assert (forall N,
-          free_vars_Hyb C \u free_vars_Hyb C \u N = free_vars_Hyb C \u N).
-intros; rewrite union_assoc; rewrite union_same; auto.
-rewrite H1; auto.
-Qed.
-
-Lemma free_vars_subset:
-forall G w Gamma M A,
-  G |= (w, Gamma) |- M ::: A ->
-  forall x, x \in free_vars_Hyb M ->
-      Mem x (concat (map (fun x => map fst_ (snd_ x)) ((w, Gamma)::G))).
-intros G w Gamma M A H; induction H; intros; rew_map; rew_concat; simpl in *.
-rewrite in_singleton in H; subst.
-rewrite Mem_app_or_eq; left. induction Gamma0; rew_map; simpl in *.
-rewrite Mem_nil_eq in HT; contradiction. destruct a; simpl in *.
-rewrite Mem_cons_eq in *; destruct HT; [inversion H; subst | ];
-[left | right]; eauto; eapply IHGamma0; auto. skip.
-Admitted.
-
-Lemma LF_to_Hyb_rel_total_L:
+Lemma LF_to_Hyb_term_R_total_L:
 forall M Gamma A G' w,
   types_LF (map snd_ G') Gamma M A ->
   LF_to_Hyb_ctx (Gamma::(map snd_ G')) ((w, Gamma)::G') ->
   exists M',
-    LF_to_Hyb_rel Gamma M A G' w M'.
+    LF_to_Hyb_term_R Gamma M A G' w M'.
 intros; generalize dependent w;
 remember (map snd_ G') as G;
-generalize dependent G';
+generalize dependent G'.
 induction H; intros; subst.
 (* hyp *)
 exists (hyp_Hyb (fte v)); econstructor; eauto using types_LF.
 (* lam *)
 assert (exists v, v \notin L \u used_vars_te_LF M \u vars_from_G_Hyb G' \u
+        used_t_vars_Hyb ((w, Gamma) :: G') \u
         from_list (map fst_ Gamma) \u used_vars_ctx_LF (Gamma::(map snd_ G')))
-  as HF by apply Fresh; destruct HF;
-destruct H0 with x G' w; auto; [eapply LF_to_Hyb_ctx_extend2_t; eauto | ].
-(*
-exists (lam_Hyb A x0); econstructor; eauto. econstructor; eauto.
+  as HF by apply Fresh; destruct HF.
+destruct H0 with x G' w as (NtoX); auto;
+[eapply LF_to_Hyb_ctx_extend2_t; eauto | ].
+exists (lam_Hyb A ([hyp_Hyb (bte 0) // fte x] NtoX));
+apply lam_LF_Hyb with (G:=map snd_ G') (L:=L); eauto.
+econstructor; eauto.
 intros; unfold open_LF in *; unfold open_t_Hyb in *.
-assert (lc_t_Hyb x0).
-  apply types_Hyb_lc_t_Hyb with (G:=G') (Gamma:=(x, A)::Gamma) (A:=B) (w:=w);
-  apply LF_to_Hyb_types in H3; auto.
-rewrite closed_subst_t_Hyb_bound with (n:=0); auto; try omega.
-replace ((v0, A) :: Gamma) with (subst_in_ctx_LF v0 x ((x,A)::Gamma)).
-replace (subst_t_LF (hyp_LF (fte v0)) (bte 0) M) with
-   (subst_t_LF (hyp_LF (fte v0)) (fte x)
-               (subst_t_LF (hyp_LF (fte x)) (bte 0) M)).
-replace G' with (map (subst_in_ctx_Hyb v0 x) G').
-replace x0 with
-  ([hyp_Hyb (fte v0) // fte x] x0).
-apply LF_to_Hyb_rel_rename_vars with ((x,A)::Gamma)
-      (subst_t_LF (hyp_LF (fte x)) (bte 0) M) G' x0
-      x v0; auto.
-rewrite closed_subst_t_Hyb_free; auto.
-(* x \notin FV x0 -- this may be tricky as x is created before x0;
-also because x0 is in a relation with M ^t^ x, and FV x0 = FV (M ^t^ x).. *)
-skip. (* !!!!! *)
-rewrite <- subst_in_bg_Hyb_no_change; auto.
-rewrite <- subst_t_neutral_free_LF; eauto.
-simpl; case_if; rewrite subst_in_ctx_LF_no_change; auto.
-*)
-(* This is the non-cheating version:
-It requires one more lemma then the one above: LF_to_Hyb_rel_subst_t_rev
-*)
-unfold open_LF in *;
-assert (LF_to_Hyb_rel ((x, A) :: Gamma)
-         (subst_t_LF (hyp_LF (fte x)) (bte 0) M) B G' w x0) by auto;
-apply LF_to_Hyb_rel_subst_t_rev with (M:=hyp_LF (fte x)) (M':=hyp_Hyb (fte x))
-                                                         (B:=A)
- in H3.
-destruct H3; exists (lam_Hyb A x1);
-apply lam_LF_Hyb with (L:=L)(G:=map snd_ G');
-[ apply t_lam_LF with (L:=L) | |]; eauto;
-intros; subst; unfold open_LF; unfold open_t_Hyb.
-replace ((v0, A) :: Gamma) with (subst_in_ctx_LF v0 x ((x,A)::Gamma)).
-replace (subst_t_LF (hyp_LF (fte v0)) (bte 0) M) with
-   (subst_t_LF (hyp_LF (fte v0)) (fte x)
-               (subst_t_LF (hyp_LF (fte x)) (bte 0) M)).
-replace G' with (map (subst_in_ctx_Hyb v0 x) G').
-replace ([hyp_Hyb (fte v0) // bte 0]x1) with
-  ([hyp_Hyb (fte v0) // fte x] ([hyp_Hyb (fte x) // bte 0] x1)).
-apply LF_to_Hyb_rel_rename_vars with ((x,A)::Gamma)
-      (subst_t_LF (hyp_LF (fte x)) (bte 0) M) G' ([hyp_Hyb (fte x) // bte 0]x1)
-      x v0; auto.
-rewrite notin_union in H2; destruct H2; rewrite <- subst_t_Hyb_neutral_free;
-auto. (* x \notin FV x1 -- this is tricky as x is created before x1 *)
-assert (~ Mem x (concat (map (fun x => map fst_ (snd_ x))
-                             ((w, Gamma)::G')))).
-  rew_map; simpl; rew_concat; rewrite Mem_app_or_eq.
-  repeat rewrite notin_union in H3; destruct H3; destruct H6; destruct H7.
-  intro; destruct H9.
-  elim H7; apply from_list_Mem; eauto.
-  skip.
-intro. apply free_vars_subset with G' w (Gamma) x1 B x in H7.
-contradiction.
-apply LF_to_Hyb_types in H4.
-
-(* PROBLEM:
-This does not type (it's open, d'uh..); for [hyp_Hyb (fte x) // bte 0]x1 version
-we cannot cheat like this (b/c x actually is in the context variables)
-Need alternatives :(
-*)
-(* This may be technical, but it should be doable with some extensions of set
-to express FV N in relation to FV [M/k]N *) skip. (* !!!!! *)
-rewrite <- subst_in_bg_Hyb_no_change; auto.
-rewrite <- subst_t_neutral_free_LF; eauto.
-simpl; case_if; rewrite subst_in_ctx_LF_no_change; auto.
-apply hyp_LF_Hyb with (G:=map snd_ G').
-constructor; auto; try apply Mem_here; apply ok_Bg_LF_fresh; auto.
-apply LF_to_Hyb_ctx_extend2_t; auto.
+apply LF_to_Hyb_term_R_renaming.
+skip. (* it is in relation, so it types, so it's lct, boooring *)
+repeat rewrite notin_union in *; repeat split;
+destruct H2; destruct H5; destruct H6; destruct H7; destruct H8;
+auto.
+auto.
 (* appl *)
 destruct IHtypes_LF1 with G' w; auto;
 destruct IHtypes_LF2 with G' w; auto;
 exists (appl_Hyb x x0); econstructor; eauto; econstructor; eauto.
 (* box *)
-remember (from_list (map fst_ (G' & (w, Gamma)))) as U.
-assert (exists (w: var), w \notin U) by apply Fresh; destruct H1;
-destruct IHtypes_LF with (G' & (w, Gamma)) x; auto;
+remember (from_list (map fst_ (G' & (w, Gamma))) \u
+                    used_w_vars_Hyb (G' & (w, Gamma))) as U.
+assert (exists (w: var), w \notin U)
+  by apply Fresh; destruct H1;
+destruct IHtypes_LF with (G' & (w, Gamma)) x as (MtoX); auto;
 [rew_map; auto | apply LF_to_Hyb_ctx_extend2_w; eauto | ].
 assert (PPermut_LF (map snd_ G' & Gamma) (Gamma :: map snd_ G'))
   by PPermut_LF_simpl;
 assert (PPermut_Hyb (G' & (w, Gamma)) ((w, Gamma) :: G'))
   by PPermut_Hyb_simpl;
-rewrite H2; rewrite H3; auto.
-assert (lc_w_Hyb x0).
+rewrite H2; rewrite H3; eauto.
+subst; auto.
+assert (lc_w_Hyb MtoX).
   apply types_Hyb_lc_w_Hyb with (G:=G' & (w, Gamma)) (Gamma:=nil) (A:=A) (w:=x);
   apply LF_to_Hyb_types in H2; auto.
-exists (box_Hyb x0); econstructor; eauto;
-[econstructor; eauto | intros]; unfold open_w_Hyb.
-assert (PPermut_Hyb (G' & (w, Gamma)) ((w, Gamma) :: G'))
-  by PPermut_Hyb_simpl;
-rewrite <- H5.
-replace (G' & (w, Gamma)) with
-  (map (subst_w_in_ctx_Hyb w0 x) (G' & (w, Gamma))).
-replace ({{fwo w0 // bwo 0}}x0) with
-  ({{fwo w0//fwo x}}{{fwo x // bwo 0}}x0).
-apply LF_to_Hyb_rel_rename_worlds with
-  (G' & (w, Gamma)) ({{fwo x // bwo 0}} x0) x x w0; eauto; try (case_if; auto).
-rewrite closed_subst_w_Hyb_bound with (n:=0); auto; try omega.
-(* Q: can I do the same cheat for lambda? (With not splitting x0) *)
-rewrite subst_w_Hyb_neutral_free; auto.
-(* Just as tricky as before, x is created before x0 *) skip.
-rewrite <- subst_w_in_bg_Hyb_no_change; subst; auto.
+exists (box_Hyb ({{bwo 0 // fwo x}}MtoX)); econstructor; eauto;
+[apply t_box_LF; eauto | intros]; unfold open_w_Hyb.
+rewrite subst_w_Hyb_neutral_bound with (n:=0); try omega; auto.
+(* this requires same approach as lambda, only with renaming of worlds *)
+skip.
 (* unbox *)
 destruct IHtypes_LF with G' w; auto;
 exists (unbox_fetch_Hyb (fwo w) x); econstructor; eauto; constructor; auto.
@@ -969,8 +870,8 @@ destruct IHtypes_LF with (G0 & (w, Gamma')) w'; auto.
 rew_map; simpl; subst; auto.
 subst. skip.
 exists (unbox_fetch_Hyb (fwo w') x).
-replace G'0 with ((w', Gamma) :: G0) by skip. (* lemma mentioned earlier *)
-apply unbox_fetch_LF_Hyb with (G:=G); eauto. skip (* from ok + rel on ctxts *).
+replace G'0 with ((w', Gamma) :: G0) by skip.
+eapply unbox_fetch_LF_Hyb with (G:=G); eauto. skip (* from ok + rel on ctxts *).
 apply t_unbox_fetch_LF with (G:=G) (Gamma:=Gamma); auto. PPermut_LF_simpl.
 skip. (* permuts *)
 replace ((w, Gamma')::G0) with (G0 & (w, Gamma')) by skip. auto.
@@ -986,21 +887,19 @@ destruct IHtypes_LF with (G0 & (w, Gamma')) w'; auto.
 rew_map; simpl; subst; auto.
 subst. skip.
 exists (get_here_Hyb (fwo w') x).
-replace G'0 with ((w', Gamma) :: G0) by skip. (* lemma mentioned earlier *)
-apply get_here_LF_Hyb with (G:=G); eauto. skip (* from ok + rel on ctxts *).
+replace G'0 with ((w', Gamma) :: G0) by skip.
+eapply get_here_LF_Hyb with (G:=G); eauto. skip (* from ok + rel on ctxts *).
 apply t_get_here_LF with (G:=G) (Gamma:=Gamma); auto. PPermut_LF_simpl.
 skip. (* permuts *)
 replace ((w, Gamma')::G0) with (G0 & (w, Gamma')) by skip. auto.
 (* letdia *)
-assert (exists x, x \notin L) by apply Fresh; destruct H2.
-destruct H0 with (((x,A)::nil) :: map snd_ G') x ((x, (x,A)::nil)::G') w; auto.
+(* Combination of lambda and box *)
 skip.
-assert ( LF_to_Hyb_rel Gamma (open_LF N (hyp_LF (fte x))) B
-         ((x, (x, A) :: nil) :: G') w x0) by auto.
-skip. (*combination of lambda and box *)
 (* letdia-get *)
-skip. (* combin. of lambda, box and unbox *)
-Qed.
+(* Combination of lambda and box *)
+skip.
+Admitted.
+*)
 
 Close Scope hybrid_is5_scope.
 Close Scope permut_scope.
